theories/aneris_lang/state_interp/state_interp_config_wp.v
@@ -36,20 +36,16 @@ Section state_interpretation.
     rewrite /config_wp. iIntros. iModIntro. iIntros (σ1 δ k σ2 ks nt Hstep) "Hσ".
     rewrite /state_interp; simplify_eq /=.
     iDestruct "Hσ" as (γm mh)
-           "(%Hhist & %Hhdomn & %Hgcoh & %Hnscoh & %Hmhcoh
+           "(%Hhist & %Hgcoh & %Hnscoh & %Hmhcoh
                     & Hnauth & Hsi & Hlcoh & Hfreeips & Hmctx & Hmres)".
     iApply step_fupd_fupd; iApply step_fupd_intro; first done.
     destruct Hstep as
         [ ip σ k Sn Sn' sh a skt R m Hm HSn Hsh HSn' Hsaddr | σ]; simpl.
     { iExists δ. iIntros "!> !>". iSplit.
-      - iPureIntro. split_and!; last by left.
-        simplify_eq. eapply message_history_evolution_deliver_message; eauto;
-        edestruct Hnscoh as (?&?&?&Hac&?); first done; eauto.
-          by symmetry; eapply Hac.
-          intros ???; edestruct Hnscoh as (?&?&?&?&?); eauto.
+      - iPureIntro. split_and!; last by left. simplify_eq.
+        eapply message_history_evolution_deliver_message; set_solver.
       - iExists γm, mh. iFrame "Hsi".
-        iSplitR; [ eauto |].
-        iSplitR; [ eauto |].
+        iSplitR; first done.
         iSplitR; [eauto using gnames_coh_update_sockets|].
         iSplitR; [eauto using network_sockets_coh_deliver_message|].
         iSplitR; [eauto using messages_history_coh_deliver_message|].
@@ -59,10 +55,11 @@ Section state_interpretation.
           rewrite /messages_resource_coh. iApply (big_sepS_mono with "Hmres").
           iIntros (??) "[Hmr|%Hmr]"; last eauto with iFrame. iLeft.
           iDestruct "Hmr" as (phi) "(Hphi & Hphi2)". eauto with iFrame. }
-    iExists δ. iIntros "!> !>". iSplit. iPureIntro. split_and!; last by left.
-    by eapply message_history_evolution_drop_message.
+    iExists δ. iIntros "!> !>". iSplit. iPureIntro.
+    split_and!; last by left.
+    eapply message_history_evolution_drop_message; set_solver.
+    (* by eapply message_history_evolution_drop_message. *)
     iExists γm, mh. iFrame. iSplitR; first done. iSplitR; first done.
-    iSplitR. iPureIntro. simpl. eauto.
     iSplitR. iPureIntro. simpl. eauto.
     iSplitR. iPureIntro. simpl. by eapply messages_history_drop_message.
     rewrite /messages_resource_coh. iApply (big_sepS_mono with "Hmres").
